siso.v
@@ -6,6 +6,43 @@ Import ListNotations.
 Require Import Setoid.
 Require Import Morphisms.
 
+(* CoInductive so: Type :=
+  | so_end    : so 
+  | so_receive: participant -> list (label*sort*so) -> so 
+  | so_send   : participant -> so -> so.
+
+CoInductive si: Type :=
+  | si_end    : si
+  | si_receive: participant -> si -> si 
+  | si_send   : participant -> list (label*sort*si) -> si.
+  
+ *)
+
+CoInductive siso: Type :=
+  | siso_end    : siso 
+  | siso_receive: participant -> (label*st.sort*siso) -> siso 
+  | siso_send   : participant -> (label*st.sort*siso) -> siso.
+
+Inductive so2siso (R: so -> siso -> Prop): so -> siso -> Prop :=
+  | so2siso_end: so2siso R so_end siso_end
+  | so2siso_rcv: forall l s x t xs p,
+                 List.In (l,s,x) xs ->
+                 R (so_receive p [(l,s,x)]) t ->
+                 so2siso R (so_receive p xs) t
+  | so2siso_snd: forall x t p,
+                 R t (siso_send p x) ->
+                 so2siso R t (siso_send p x).
+
+Inductive si2siso (R: si -> siso -> Prop): si -> siso -> Prop :=
+  | si2siso_end: si2siso R si_end siso_end
+  | si2siso_rcv: forall x t p,
+                 R t (siso_receive p x) ->
+                 si2siso R t (siso_receive p x)
+  | si2siso_snd: forall l s x t xs p,
+                 List.In (l,s,x) xs ->
+                 R (si_send p [(l,s,x)]) t ->
+                 si2siso R (si_send p xs) t.
+
 Inductive st2siso (R: st -> st -> Prop): st -> st -> Prop :=
   | st2siso_end: st2siso R st_end st_end
   | st2siso_rcv: forall l s x t xs p,
@@ -33,6 +70,8 @@ Proof. unfold monotone2.
 Qed.
 
 Definition st2sisoC s1 s2 := paco2 (st2siso) bot2 s1 s2.
+Definition so2sisoC s1 s2 := paco2 (so2siso) bot2 s1 s2.
+Definition si2sisoC s1 s2 := paco2 (si2siso) bot2 s1 s2.
 
 #[export]
 Declare Instance Equivalence_st2siso : Equivalence st2sisoC.
@@ -45,6 +84,18 @@ Definition siso_id (t: st): st :=
   end.
 
 Lemma siso_eq: forall t, t = siso_id t.
+Proof. intro t.
+       destruct t; try easy.
+Defined.
+
+Definition siso_idA (t: siso): siso :=
+  match t with
+    | siso_receive p a => siso_receive p a
+    | siso_send p a    => siso_send p a
+    | siso_end         => siso_end
+  end.
+
+Lemma siso_eqA: forall t, t = siso_idA t.
 Proof. intro t.
        destruct t; try easy.
 Defined.
@@ -78,6 +129,13 @@ CoFixpoint act (t: st): coseq (participant * string) :=
   match t with
     | st_receive p [(l,s,w')] => Delay (cocons (p, "?"%string) (act w'))
     | st_send p [(l,s,w')]    => Delay (cocons (p, "!"%string) (act w'))
+    | _                       => Delay conil
+  end.
+
+CoFixpoint actC (t: siso): coseq (participant * string) :=
+  match t with
+    | siso_receive p (l,s,w') => Delay (cocons (p, "?"%string) (actC w'))
+    | siso_send p (l,s,w')    => Delay (cocons (p, "!"%string) (actC w'))
     | _                       => Delay conil
   end.
 
@@ -205,12 +263,25 @@ CoFixpoint merge_ap_cont (p: participant) (a: Ap p) (w: st): st :=
     | ap_end              => w
   end.
 
+CoFixpoint merge_ap_contB (p: participant) (a: Ap p) (w: siso): siso :=
+  match a with
+    | ap_receive q H l s  => siso_receive q (l,s,w)
+    | ap_merge q H l s w' => siso_receive q (l,s,(merge_ap_contB p w' w))
+    | ap_end              => w
+  end.
+
 Fixpoint merge_ap_contn (p: participant) (a: Ap p) (w: st) (n: nat): st :=
   match n with
     | O    => w
     | S k  => merge_ap_cont p a (merge_ap_contn p a w k)
   end.
 
+Fixpoint merge_ap_contnB (p: participant) (a: Ap p) (w: siso) (n: nat): siso :=
+  match n with
+    | O    => w
+    | S k  => merge_ap_contB p a (merge_ap_contnB p a w k)
+  end.
+  
 Fixpoint merge_ap_contnA (p: participant) (a: Ap p) (w: st) (n: nat): st :=
   match n with
     | O    => w
@@ -301,10 +372,25 @@ CoFixpoint merge_bp_cont (p: participant) (b: Bp p) (w: st): st :=
     | bp_end             => w
   end.
 
+CoFixpoint merge_bp_contB (p: participant) (b: Bp p) (w: siso): siso :=
+  match b with 
+    | bp_receivea q l s  => siso_receive q (l,s,w)
+    | bp_send q x l s    => siso_send q (l,s,w)
+    | bp_mergea q l s c  => siso_receive q (l,s,(merge_bp_contB p c w))
+    | bp_merge q x l s c => siso_send q (l,s,(merge_bp_contB p c w))
+    | bp_end             => w
+  end.
+
 Fixpoint merge_bp_contn (p: participant) (b: Bp p) (w: st) (n: nat): st :=
   match n with
     | O    => w
     | S k  => merge_bp_cont p b (merge_bp_contn p b w k)
+  end.
+
+Fixpoint merge_bp_contnB (p: participant) (b: Bp p) (w: siso) (n: nat): siso :=
+  match n with
+    | O    => w
+    | S k  => merge_bp_contB p b (merge_bp_contnB p b w k)
   end.
 
 Fixpoint bpList (p: participant) (b: Bp p): list (Bp p) :=
@@ -700,6 +786,8 @@ Inductive cosetIncR: list (participant * string) -> coseq (participant * string)
 
 Definition act_eq (w w': st) := forall a, CoIn a (act w) <-> CoIn a (act w').
 
+Definition act_eqB (w w': siso) := forall a, CoIn a (actC w) <-> CoIn a (actC w').
+
 Inductive refinementR (seq: st -> st -> Prop): st -> st -> Prop :=
   | _sref_in : forall w w' p l s s',
                       subsort s' s -> 
@@ -778,3 +866,35 @@ forall w w' p l s s' a n,
                       act_eq w (merge_bp_contn p b w' n) ->
                       refinementR seq (st_send p [(l,s,w)]) (merge_bp_contn p b (st_send p [(l,s',w')]) n)
 *)
+
+Inductive refinementRA (seq: siso -> siso -> Prop): siso -> siso -> Prop :=
+  | _sref_inA : forall w w' p l s s',
+                       subsort s' s -> 
+                       seq w w' ->
+                       refinementRA seq (siso_receive p (l,s,w)) (siso_receive p (l,s',w'))
+
+  | _sref_outA: forall w w' p l s s',
+                       subsort s s' ->
+                       seq w w' ->
+                       refinementRA seq (siso_send p (l,s,w)) (siso_send p (l,s',w'))
+
+  | _sref_aA  : forall w w' p l s s' a n,
+                       subsort s s' ->
+                       seq w (merge_ap_contnB p a w' n)  ->
+                       act_eqB w (merge_ap_contnB p a w' n) ->
+                       refinementRA seq (siso_receive p (l,s',w)) (merge_ap_contnB p a (siso_receive p (l,s,w')) n)
+
+  | _sref_bA  : forall w w' p l s s' b n,
+                      subsort s s' ->
+                      seq w (merge_bp_contnB p b w' n) ->
+                      act_eqB w (merge_bp_contnB p b w' n) ->
+                      refinementRA seq (siso_send p (l,s,w)) (merge_bp_contnB p b (siso_send p (l,s',w')) n)
+  | _sref_endA: refinementRA seq siso_end siso_end.
+
+Definition refinementRAC: siso -> siso -> Prop := fun s1 s2 => paco2 refinementRA bot2 s1 s2.
+
+Notation "x '~<A' y" := (refinementRAC x y) (at level 50, left associativity).
+
+
+
+
