so.v
@@ -16,6 +16,18 @@ CoInductive so: Type :=
 
 Local Open Scope list_scope.
 
+Inductive st2soA (R: st -> so -> Prop): st -> so -> Prop :=
+  | st2soA_end: st2soA R st_end so_end
+  | st2soA_snd: forall l s x t xs p,
+                List.In (l,s,x) xs ->
+                R (st_send p [(l,s,x)]) t ->
+                st2soA R (st_send p xs) t
+  | st2soA_rcv: forall p l s t xs ys,
+                List.Forall (fun u => R (fst u) (snd u)) (zip xs ys) ->
+                List.In t ys ->
+                R (st_receive p (zip (zip l s) xs)) t ->
+                st2soA R (st_receive p (zip (zip l s) xs)) t.
+
 Inductive st2so (R: st -> st -> Prop): st -> st -> Prop :=
   | st2so_end: st2so R st_end st_end
   | st2so_snd: forall l s x t xs p,
@@ -49,6 +61,8 @@ Proof. unfold monotone2.
 Qed.
 
 Definition st2soC s1 s2 := paco2 (st2so) bot2 s1 s2.
+Definition st2soCA s1 s2 := paco2 (st2soA) bot2 s1 s2.
 
 #[export]
 Declare Instance Equivalence_st2so : Equivalence st2soC.
+
